update syntax

Metamath/Translate.lean
@@ -37,15 +37,15 @@ structure VR where (type : CN) (i : Nat)
 deriving DecidableEq
 
 inductive Sym
-| const (c : CN)
-| var (n : VR)
-deriving Inhabited, DecidableEq
+  | const (c : CN)
+  | var (n : VR)
+  deriving Inhabited, DecidableEq
 open Sym
 
 instance : Coe String Sym := ⟨const⟩
 def Sym.isVar : Sym → Bool
-| const _ => false
-| var _ => true
+  | const _ => false
+  | var _ => true
 
 def Expr := List Sym
 def VR.expr (v : VR) : Expr := [var v]
@@ -61,63 +61,63 @@ def Expr.mem (e : Expr) (v : VR) : Prop := var v ∈ e
 scoped notation:50 a:51 " ∈' " b:51 => Expr.mem b a
 
 def Expr.vars : Expr → List VR
-| [] => []
-| const _ :: e => vars e
-| var v :: e => v :: vars e
+  | [] => []
+  | const _ :: e => vars e
+  | var v :: e => v :: vars e
 
 def Expr.subst (σ : VR → Expr) : Expr → Expr
-| [] => []
-| const c :: e => const c :: subst σ e
-| var v :: e => σ v ++ subst σ e
+  | [] => []
+  | const c :: e => const c :: subst σ e
+  | var v :: e => σ v ++ subst σ e
 
 theorem Expr.subst_id : (e : Expr) → Expr.subst VR.expr e = e
-| [] => rfl
-| const c :: e => congrArg (const c :: .) (subst_id e)
-| var v :: e => congrArg (var v :: .) (subst_id e)
+  | [] => rfl
+  | const c :: e => congrArg (const c :: .) (subst_id e)
+  | var v :: e => congrArg (var v :: .) (subst_id e)
 
 theorem Expr.subst_append (σ) : (e₁ e₂ : Expr) → Expr.subst σ (e₁ ++ e₂) = e₁.subst σ ++ e₂.subst σ
-| [], _ => rfl
-| const c :: (e₁ : Expr), e₂ => by
-  rw [subst, List.cons_append, subst, subst_append ..]; rfl
-| var v :: e, e₂ => by
-  rw [List.cons_append]; simp only [Expr.subst]; rw [List.append_assoc, subst_append ..]
+  | [], _ => rfl
+  | const c :: (e₁ : Expr), e₂ => by
+    rw [subst, List.cons_append, subst, subst_append ..]; rfl
+  | var v :: e, e₂ => by
+    rw [List.cons_append]; simp only [Expr.subst]; rw [List.append_assoc, subst_append ..]
 
 theorem Expr.mem_subst {σ a} : {e : Expr} → a ∈' Expr.subst σ e → ∃ b, b ∈' e ∧ a ∈' σ b
-| const _ :: _, .tail _ h => let ⟨b, h₁, h₂⟩ := mem_subst h; ⟨b, .tail _ h₁, h₂⟩
-| var v :: _, h =>
-  match List.mem_append.1 h with
-  | Or.inl h => ⟨v, .head _, h⟩
-  | Or.inr h => let ⟨b, h₁, h₂⟩ := mem_subst h; ⟨b, .tail _ h₁, h₂⟩
+  | const _ :: _, .tail _ h => let ⟨b, h₁, h₂⟩ := mem_subst h; ⟨b, .tail _ h₁, h₂⟩
+  | var v :: _, h =>
+    match List.mem_append.1 h with
+    | Or.inl h => ⟨v, .head _, h⟩
+    | Or.inr h => let ⟨b, h₁, h₂⟩ := mem_subst h; ⟨b, .tail _ h₁, h₂⟩
 
 def subst.trans (σ σ' : VR → Expr) (v : VR) : Expr := (σ v).subst σ'
 
 theorem Expr.subst_tr (σ σ' : VR → Expr) : (e : Expr) →
-  e.subst (subst.trans σ σ') = (e.subst σ).subst σ'
-| [] => rfl
-| const c :: e => congrArg (const c :: .) (subst_tr _ _ e)
-| var v :: e => by simp only [subst]; rw [subst_append, subst_tr _ _ e]; rfl
+    e.subst (subst.trans σ σ') = (e.subst σ).subst σ'
+  | [] => rfl
+  | const c :: e => congrArg (const c :: .) (subst_tr _ _ e)
+  | var v :: e => by simp only [subst]; rw [subst_append, subst_tr _ _ e]; rfl
 
 def Formula := CN × Expr
 
 def Formula.subst (σ : VR → Expr) : Formula → Formula
-| (c, e) => (c, e.subst σ)
+  | (c, e) => (c, e.subst σ)
 
 theorem Formula.subst_id : (e : Formula) → Formula.subst VR.expr e = e
-| (c, e) => congrArg (c, .) e.subst_id
+  | (c, e) => congrArg (c, .) e.subst_id
 
 theorem Formula.subst_tr (σ σ' : VR → Expr) : (e : Formula) →
-  e.subst (subst.trans σ σ') = (e.subst σ).subst σ'
-| (c, e) => congrArg (c, .) (e.subst_tr _ _)
+    e.subst (subst.trans σ σ') = (e.subst σ).subst σ'
+  | (c, e) => congrArg (c, .) (e.subst_tr _ _)
 
 def VR.vhyp (v : VR) : Formula := (v.type, [var v])
 instance : Coe VR Formula := ⟨VR.vhyp⟩
 
 def Expr.δ (a b : Expr) : Bool :=
-a.all fun
-| const _ => true
-| var a => b.all fun
+  a.all fun
   | const _ => true
-  | var b => a != b
+  | var a => b.all fun
+    | const _ => true
+    | var b => a != b
 
 structure DJ where
   disj : VR → VR → Prop
@@ -133,47 +133,47 @@ theorem DJ.ne (dj : DJ) {a b} (h : dj a b) : a ≠ b :=
   fun e => by cases e; exact dj.irr h
 
 theorem DJ.ext : {dj₁ dj₂ : DJ} → (∀ a b, dj₁ a b ↔ dj₂ a b) → dj₁ = dj₂
-| ⟨dj₁, _, _⟩, ⟨dj₂, _, _⟩, h =>
-  have : dj₁ = dj₂ := funext fun a => funext fun b => propext (h a b)
-  by cases this; rfl
+  | ⟨dj₁, _, _⟩, ⟨dj₂, _, _⟩, h =>
+    have : dj₁ = dj₂ := funext fun a => funext fun b => propext (h a b)
+    by cases this; rfl
 
 theorem DJ.le_antisymm {dj₁ dj₂ : DJ} (H₁ : dj₁ ≤ dj₂) (H₂ : dj₂ ≤ dj₁) : dj₁ = dj₂ :=
   DJ.ext fun _ _ => ⟨H₁ _ _, H₂ _ _⟩
 
-def DJ.mk' (disj : List (VR × VR)) : DJ :=
-{ disj := fun a b => a ≠ b ∧ ((a, b) ∈ disj ∨ (b, a) ∈ disj)
+def DJ.mk' (disj : List (VR × VR)) : DJ where
+  disj := fun a b => a ≠ b ∧ ((a, b) ∈ disj ∨ (b, a) ∈ disj)
   irr := fun h => h.1 rfl
-  symm := fun ⟨h, h'⟩ => ⟨h.symm, h'.symm⟩ }
+  symm := fun ⟨h, h'⟩ => ⟨h.symm, h'.symm⟩
 
 def Expr.disjoint (dj : DJ) (e₁ e₂ : Expr) : Prop :=
   ∀ a b, a ∈' e₁ → b ∈' e₂ → dj a b
 
 theorem Expr.disjoint.mono {dj₁ dj₂ : DJ} (h : dj₁ ≤ dj₂) {e₁ e₂}
-  (H : Expr.disjoint dj₁ e₁ e₂) : Expr.disjoint dj₂ e₁ e₂ :=
+    (H : Expr.disjoint dj₁ e₁ e₂) : Expr.disjoint dj₂ e₁ e₂ :=
   fun a b ha hb => h _ _ (H a b ha hb)
 
 def DJ.subst (σ : VR → Expr) (dj dj' : DJ) :=
   ∀ a b, dj a b → (σ a).disjoint dj' (σ b)
 
 theorem DJ.subst.mono {σ : VR → Expr} {dj₁ dj₂ dj₁' dj₂' : DJ}
-  (h : dj₂ ≤ dj₁) (h' : dj₁' ≤ dj₂') (H : dj₁.subst σ dj₁') : dj₂.subst σ dj₂' :=
+    (h : dj₂ ≤ dj₁) (h' : dj₁' ≤ dj₂') (H : dj₁.subst σ dj₁') : dj₂.subst σ dj₂' :=
   fun _ _ d => Expr.disjoint.mono h' (H _ _ (h _ _ d))
 
 def DJ.trim (dj : DJ) (P : VR → Prop) : DJ :=
-{ disj := fun x y => dj x y ∧ P x ∧ P y
-  irr := fun x => dj.irr x.1
-  symm := fun ⟨h₁, h₂, h₃⟩ => ⟨dj.symm h₁, h₃, h₂⟩ }
+  { disj := fun x y => dj x y ∧ P x ∧ P y
+    irr := fun x => dj.irr x.1
+    symm := fun ⟨h₁, h₂, h₃⟩ => ⟨dj.symm h₁, h₃, h₂⟩ }
 
 theorem DJ.trim.mono {dj₁ dj₂ : DJ} (hdj : dj₁ ≤ dj₂) {P Q : VR → Prop}
-  (pq : ∀ x, P x → Q x) : dj₁.trim P ≤ dj₂.trim Q :=
+    (pq : ∀ x, P x → Q x) : dj₁.trim P ≤ dj₂.trim Q :=
   fun _ _ ⟨h, ha, hb⟩ => ⟨hdj _ _ h, pq _ ha, pq _ hb⟩
 
 def DJ.trimmed (dj : DJ) (P : VR → Prop) : Prop :=
   ∀ a b, dj a b → P a ∧ P b
 
 theorem DJ.trimmed.mono (dj : DJ) {P Q : VR → Prop}
-  (h : ∀ x, P x → Q x) (H : dj.trimmed P) : dj.trimmed Q
-| a, b, d => let ⟨h₁, h₂⟩ := H a b d; ⟨h _ h₁, h _ h₂⟩
+    (h : ∀ x, P x → Q x) (H : dj.trimmed P) : dj.trimmed Q
+  | a, b, d => let ⟨h₁, h₂⟩ := H a b d; ⟨h _ h₁, h _ h₂⟩
 
 theorem DJ.trim_le_self (dj : DJ) (P : VR → Prop) : dj.trim P ≤ dj := fun _ _ d => d.1
 
@@ -182,13 +182,13 @@ theorem DJ.trim.trimmed (dj : DJ) (P : VR → Prop) : (dj.trim P).trimmed P := f
 theorem DJ.trimmed.trim_eq {dj : DJ} {P} (h : dj.trimmed P) : dj.trim P = dj :=
   DJ.ext fun _ _ => ⟨fun h => h.1, fun h' => ⟨h', h _ _ h'⟩⟩
 
-def DJ.untrim (dj : DJ) (P : VR → Prop) : DJ :=
-{ disj := fun x y => x ≠ y ∧ (P x → P y → dj x y)
+def DJ.untrim (dj : DJ) (P : VR → Prop) : DJ where
+  disj := fun x y => x ≠ y ∧ (P x → P y → dj x y)
   irr := fun x => x.1 rfl
-  symm := fun ⟨h₁, h₂⟩ => ⟨h₁.symm, fun x y => dj.symm (h₂ y x)⟩ }
+  symm := fun ⟨h₁, h₂⟩ => ⟨h₁.symm, fun x y => dj.symm (h₂ y x)⟩
 
 theorem DJ.untrim.mono {dj₁ dj₂ : DJ} (hdj : dj₁ ≤ dj₂) {P Q : VR → Prop}
-  (qp : ∀ x, Q x → P x) : dj₁.untrim P ≤ dj₂.untrim Q :=
+    (qp : ∀ x, Q x → P x) : dj₁.untrim P ≤ dj₂.untrim Q :=
   fun _ _ ⟨h₁, h₂⟩ => ⟨h₁, fun ha hb => hdj _ _ (h₂ (qp _ ha) (qp _ hb))⟩
 
 theorem DJ.trim_le {dj₁ dj₂ : DJ} {P} : dj₁.trim P ≤ dj₂ ↔ dj₁ ≤ dj₂.untrim P :=
@@ -229,8 +229,8 @@ def Statement.vars (s : Statement) : List VR :=
   (s.fmla :: s.ctx.hyps).flatMap fun e => e.2.vars
 
 theorem Statement.vars.mono' {s₁ s₂ : Statement}
-  (H : ∀ a, a ∈ s₁.ctx.hyps → a ∈ s₂.ctx.hyps) (H₂ : s₁.fmla = s₂.fmla)
-  (v) : v ∈ s₁.vars → v ∈ s₂.vars := by
+    (H : ∀ a, a ∈ s₁.ctx.hyps → a ∈ s₂.ctx.hyps) (H₂ : s₁.fmla = s₂.fmla)
+    (v) : v ∈ s₁.vars → v ∈ s₂.vars := by
   simp only [vars, List.mem_flatMap, List.mem_cons, H₂]
   exact fun ⟨a, b, c⟩ => ⟨a, b.imp_right (H _), c⟩
 
@@ -240,7 +240,7 @@ theorem Statement.vars.mono {s₁ s₂ : Statement} (H : s₁ ≤ s₂) : ∀ v,
 def Statement.trim (s : Statement) : Statement :=
   ⟨⟨s.ctx.hyps, s.ctx.dj.trim fun v => v ∈ s.vars⟩, s.fmla⟩
 
-def Statement.untrim' (s : Statement) (P : VR → Prop): Statement :=
+def Statement.untrim' (s : Statement) (P : VR → Prop) : Statement :=
   ⟨⟨s.ctx.hyps, s.ctx.dj.untrim P⟩, s.fmla⟩
 def Statement.untrim (s : Statement) : Statement := s.untrim' fun v => v ∈ s.vars
 
@@ -255,10 +255,10 @@ theorem Statement.trim.mono {s₁ s₂ : Statement} (h : s₁ ≤ s₂) : s₁.t
   ⟨⟨h.1.1, DJ.trim.mono h.1.2 (Statement.vars.mono h)⟩, h.2⟩
 
 theorem Statement.untrim'.mono {s₁ s₂ : Statement} {P Q}
-  (H : ∀ x, Q x → P x) (h : s₁ ≤ s₂) : s₁.untrim' P ≤ s₂.untrim' Q :=
+    (H : ∀ x, Q x → P x) (h : s₁ ≤ s₂) : s₁.untrim' P ≤ s₂.untrim' Q :=
   ⟨⟨h.1.1, DJ.untrim.mono h.1.2 H⟩, h.2⟩
 theorem Statement.untrim.mono {s₁ s₂ : Statement}
-  (H : s₁.ctx.hyps = s₂.ctx.hyps) (h : s₁ ≤ s₂) : s₁.untrim ≤ s₂.untrim :=
+    (H : s₁.ctx.hyps = s₂.ctx.hyps) (h : s₁ ≤ s₂) : s₁.untrim ≤ s₂.untrim :=
   Statement.untrim'.mono (Statement.vars.mono' (by rw [H]; exact fun _ => id) h.2.symm) h
 
 theorem Statement.trim_vars (s : Statement) : s.trim.vars = s.vars := rfl
@@ -272,7 +272,7 @@ theorem Statement.untrim_trim (s : Statement) : s.trim.untrim = s.untrim := by
   simp only [untrim, untrim', trim_vars]; simp only [trim, DJ.untrim_trim]
 
 theorem Statement.trim_le {s₁ s₂ : Statement} (e : s₁.vars = s₂.vars) :
-  s₁.trim.ctx ≤ s₂.ctx ↔ s₁.ctx ≤ s₂.untrim.ctx :=
+    s₁.trim.ctx ≤ s₂.ctx ↔ s₁.ctx ≤ s₂.untrim.ctx :=
   ⟨fun ⟨h₁, h₂⟩ => ⟨h₁, DJ.trim_le.1 $ by rw [← e]; exact h₂⟩,
    fun ⟨h₁, h₂⟩ => ⟨h₁, DJ.trim_le.2 $ by rw [e]; exact h₂⟩⟩
 
@@ -281,17 +281,17 @@ def Statement.trimmed (s : Statement) : Prop := s.ctx.dj.trimmed fun v => v ∈ 
 theorem Statement.trim.trimmed (s : Statement) : s.trim.trimmed := DJ.trim.trimmed _ _
 
 theorem Statement.trimmed.trim_eq : {s : Statement} → s.trimmed → s.trim = s
-| ⟨⟨a, b⟩, c⟩, h => by simp only [trim]; rw [DJ.trimmed.trim_eq h]
+  | ⟨⟨a, b⟩, c⟩, h => by simp only [trim]; rw [DJ.trimmed.trim_eq h]
 
 inductive Provable (axs : Statement → Prop) (Γ : Context) : Formula → Prop
-| hyp (h) : h ∈ Γ.hyps → Provable axs Γ h
-| var (v:VR) : Provable axs Γ v
-| ax (σ) {ax} : axs ax → ax.ctx.dj.subst σ Γ.dj →
-  (∀ h, h ∈ ax.ctx.hyps ∨ (∃ v:VR, h = v) → Provable axs Γ (h.subst σ)) →
-  Provable axs Γ (ax.fmla.subst σ)
+  | hyp (h) : h ∈ Γ.hyps → Provable axs Γ h
+  | var (v:VR) : Provable axs Γ v
+  | ax (σ) {ax} : axs ax → ax.ctx.dj.subst σ Γ.dj →
+    (∀ h, h ∈ ax.ctx.hyps ∨ (∃ v:VR, h = v) → Provable axs Γ (h.subst σ)) →
+    Provable axs Γ (ax.fmla.subst σ)
 
 theorem Provable.mono {axs₁ axs₂} (haxs : ∀ a, axs₁ a → axs₂ a)
-  {Γ₁ Γ₂} (hΓ : Γ₁ ≤ Γ₂) {e} (pr : Provable axs₁ Γ₁ e) : Provable axs₂ Γ₂ e := by
+    {Γ₁ Γ₂} (hΓ : Γ₁ ≤ Γ₂) {e} (pr : Provable axs₁ Γ₁ e) : Provable axs₂ Γ₂ e := by
   induction pr with
   | hyp e h => exact hyp e (hΓ.1 _ h)
   | var v => exact var v
@@ -302,8 +302,8 @@ def Statement.provable' (axs : Statement → Prop) (s : Statement) : Prop :=
   Provable axs s.ctx s.fmla
 
 theorem Statement.provable'.mono {axs₁ axs₂} (haxs : ∀ a, axs₁ a → axs₂ a) :
-  {s₁ s₂ : Statement} → s₁ ≤ s₂ → s₁.provable' axs₁ → s₂.provable' axs₂
-| ⟨_Γ₁, _⟩, ⟨_Γ₂, _⟩, ⟨hΓ, rfl⟩ => Provable.mono haxs hΓ
+    {s₁ s₂ : Statement} → s₁ ≤ s₂ → s₁.provable' axs₁ → s₂.provable' axs₂
+  | ⟨_Γ₁, _⟩, ⟨_Γ₂, _⟩, ⟨hΓ, rfl⟩ => Provable.mono haxs hΓ
 
 def Statement.provable (axs : Statement → Prop) (s : Statement) : Prop :=
   s.untrim.provable' axs
@@ -317,8 +317,8 @@ def Statement.provable (axs : Statement → Prop) (s : Statement) : Prop :=
 theorem Statement.provable'.of {axs} {s : Statement} (h : s.provable' axs) : s.provable axs :=
   h.mono (fun _ => id) (self_le_untrim _)
 
-theorem Statement.provable.trim {axs} {s : Statement} : s.trim.provable axs ↔ s.provable axs :=
-  by simp only [provable, untrim_trim]
+theorem Statement.provable.trim {axs} {s : Statement} : s.trim.provable axs ↔ s.provable axs := by
+  simp only [provable, untrim_trim]
 
 theorem Provable.ax_self (axs : Statement → Prop) {ax} (H : axs ax) : ax.provable' axs := by
   have := Provable.ax (Γ := ax.ctx) VR.expr H ?disj ?hyp
@@ -334,9 +334,9 @@ theorem Provable.ax_self (axs : Statement → Prop) {ax} (H : axs ax) : ax.prova
     | _, Or.inr ⟨v, rfl⟩ => exact Provable.var v
 
 theorem Provable.trans' {axs Γ} (σ) {Γ' fmla} (pr : Provable axs Γ' fmla)
-  (dj : Γ'.dj.subst σ Γ.dj)
-  (hh : ∀ h, h ∈ Γ'.hyps ∨ (∃ v:VR, h = v) → Provable axs Γ (h.subst σ)) :
-  Provable axs Γ (fmla.subst σ) := by
+    (dj : Γ'.dj.subst σ Γ.dj)
+    (hh : ∀ h, h ∈ Γ'.hyps ∨ (∃ v:VR, h = v) → Provable axs Γ (h.subst σ)) :
+    Provable axs Γ (fmla.subst σ) := by
   induction pr with
   | hyp f h => exact hh _ (Or.inl h)
   | var v => exact hh _ (Or.inr ⟨v, rfl⟩)
@@ -352,14 +352,14 @@ theorem Provable.trans' {axs Γ} (σ) {Γ' fmla} (pr : Provable axs Γ' fmla)
     focus { intros f; rw [Formula.subst_tr]; refine IH _ }
 
 theorem Provable.trans'' {axs Γ σ} (s : Statement) : s.provable' axs →
-  s.ctx.dj.subst σ Γ.dj →
-  (∀ h, h ∈ s.ctx.hyps ∨ (∃ v:VR, h = v) → Provable axs Γ (h.subst σ)) →
-  Provable axs Γ (s.fmla.subst σ) :=
+    s.ctx.dj.subst σ Γ.dj →
+    (∀ h, h ∈ s.ctx.hyps ∨ (∃ v:VR, h = v) → Provable axs Γ (h.subst σ)) →
+    Provable axs Γ (s.fmla.subst σ) :=
   Provable.trans' (axs := axs) σ
 
 def subst_of : List (VR × Expr) → VR → Expr
-| [], v => v
-| (a, e)::l, v => if a = v then e else subst_of l v
+  | [], v => v
+  | (a, e)::l, v => if a = v then e else subst_of l v
 
 class Subst (σ : VR → Expr) (e : Expr) (e' : outParam Expr) where (out : e.subst σ = e')
 
@@ -377,7 +377,7 @@ def subst.ok (axs Γ) (σ : VR → Expr) := ∀ v, Provable axs Γ (v.type, σ v
 
 theorem subst.ok.nil {axs Γ} : subst.ok axs Γ (subst_of []) := Provable.var
 theorem subst.ok.cons {axs Γ e σ} (x) (h₁ : Provable axs Γ (x.type, e))
-  (h₂ : subst.ok axs Γ (subst_of σ)) : subst.ok axs Γ (subst_of ((x, e)::σ)) := by
+    (h₂ : subst.ok axs Γ (subst_of σ)) : subst.ok axs Γ (subst_of ((x, e)::σ)) := by
   intro v
   simp only [subst_of]
   cases Decidable.em (x = v) with simp [h]
@@ -385,11 +385,11 @@ theorem subst.ok.cons {axs Γ e σ} (x) (h₁ : Provable axs Γ (x.type, e))
   | inr h => exact h₂ v
 
 theorem Provable.thm {axs} {Γ : Context}
-  {σ : VR → Expr} {dj hyps c s} (pr : Provable axs (Context.mk' dj hyps) (c, s))
-  (hv : subst.ok axs Γ σ)
-  (dj : (DJ.mk' dj).subst σ Γ.dj)
-  (hh : ∀ h, h ∈ hyps → Provable axs Γ (h.subst σ))
-  {e} [inst : Subst σ s e] : Provable axs Γ (c, e) := by
+    {σ : VR → Expr} {dj hyps c s} (pr : Provable axs (Context.mk' dj hyps) (c, s))
+    (hv : subst.ok axs Γ σ)
+    (dj : (DJ.mk' dj).subst σ Γ.dj)
+    (hh : ∀ h, h ∈ hyps → Provable axs Γ (h.subst σ))
+    {e} [inst : Subst σ s e] : Provable axs Γ (c, e) := by
   rw [← inst.out]
   exact Metamath.Provable.trans' σ pr dj fun
     | f, Or.inl h => hh _ h
@@ -399,22 +399,22 @@ theorem Provable.thm {axs} {Γ : Context}
 
 theorem DJ_nil {σ dj'} : (DJ.mk' []).subst σ dj' | _, _, h => nomatch h
 theorem DJ_cons {a b l σ dj'}
-  (h₁ : (σ a).disjoint dj' (σ b))
-  (h₂ : (DJ.mk' l).subst σ dj') : (DJ.mk' ((a, b) :: l)).subst σ dj'
-| _, _, ⟨_, Or.inl (List.Mem.head _)⟩ => h₁
-| _, _, ⟨_, Or.inr (List.Mem.head _)⟩ => fun x y hx hy => dj'.symm (h₁ y x hy hx)
-| _, _, ⟨h, Or.inl (List.Mem.tail _ h')⟩ => h₂ _ _ ⟨h, Or.inl h'⟩
-| _, _, ⟨h, Or.inr (List.Mem.tail _ h')⟩ => h₂ _ _ ⟨h, Or.inr h'⟩
+    (h₁ : (σ a).disjoint dj' (σ b))
+    (h₂ : (DJ.mk' l).subst σ dj') : (DJ.mk' ((a, b) :: l)).subst σ dj'
+  | _, _, ⟨_, Or.inl (List.Mem.head _)⟩ => h₁
+  | _, _, ⟨_, Or.inr (List.Mem.head _)⟩ => fun x y hx hy => dj'.symm (h₁ y x hy hx)
+  | _, _, ⟨h, Or.inl (List.Mem.tail _ h')⟩ => h₂ _ _ ⟨h, Or.inl h'⟩
+  | _, _, ⟨h, Or.inr (List.Mem.tail _ h')⟩ => h₂ _ _ ⟨h, Or.inr h'⟩
 
 theorem HH_nil {axs Γ σ} : ∀ h:Formula, h ∈ [] → Provable axs Γ (h.subst σ)
-| _, h => nomatch h
+  | _, h => nomatch h
 
 theorem HH_cons {axs Γ σ c f hyps}
-  {e} [Subst σ f e] (h₁ : Provable axs Γ (c, e))
-  (h₂ : ∀ h:Formula, h ∈ hyps → Provable axs Γ (h.subst σ)) :
-  ∀ h:Formula, h ∈ (c, f)::hyps → Provable axs Γ (h.subst σ)
-| _, .head _ => by rw [← @Subst.out σ f e] at h₁; exact h₁
-| _, .tail _ h => h₂ _ h
+    {e} [Subst σ f e] (h₁ : Provable axs Γ (c, e))
+    (h₂ : ∀ h:Formula, h ∈ hyps → Provable axs Γ (h.subst σ)) :
+    ∀ h:Formula, h ∈ (c, f)::hyps → Provable axs Γ (h.subst σ)
+  | _, .head _ => by rw [← @Subst.out σ f e] at h₁; exact h₁
+  | _, .tail _ h => h₂ _ h
 
 class Typed (axs : outParam _) (c : outParam CN) (e : Expr) where
   type Γ : Provable axs Γ (c, e)
@@ -467,46 +467,46 @@ abbrev Provable := Metamath.Provable axs
 abbrev Typed := Metamath.Typed axs
 
 instance tze : Typed "term" ze :=
-⟨fun _Γ => (Provable.ax_self axs (.head _)).thm subst.ok.nil DJ_nil HH_nil⟩
+  ⟨fun _Γ => (Provable.ax_self axs (.head _)).thm subst.ok.nil DJ_nil HH_nil⟩
 
 instance tpl {t r} [Typed "term" t] [Typed "term" r] :
-  Typed "term" (pl t r) :=
-⟨fun _Γ =>
-  have : Subst (subst_of [(vt, t), (vr, r)]) vt t := ⟨List.append_nil _⟩
-  have : Subst (subst_of [(vt, t), (vr, r)]) vr r := ⟨List.append_nil _⟩
-  (Provable.ax_self axs (.tail _ <| .head _)).thm
-    (subst.ok.cons vt t.ty $ subst.ok.cons vr r.ty subst.ok.nil)
-    DJ_nil HH_nil⟩
+    Typed "term" (pl t r) :=
+  ⟨fun _Γ =>
+    have : Subst (subst_of [(vt, t), (vr, r)]) vt t := ⟨List.append_nil _⟩
+    have : Subst (subst_of [(vt, t), (vr, r)]) vr r := ⟨List.append_nil _⟩
+    (Provable.ax_self axs (.tail _ <| .head _)).thm
+      (subst.ok.cons vt t.ty $ subst.ok.cons vr r.ty subst.ok.nil)
+      DJ_nil HH_nil⟩
 
 instance weq {t r} [Typed "term" t] [Typed "term" r] :
-  Typed "wff" (eq t r) :=
-⟨fun _Γ =>
-  have : Subst (subst_of [(vt, t), (vr, r)]) vt t := ⟨List.append_nil _⟩
-  have : Subst (subst_of [(vt, t), (vr, r)]) vr r := ⟨List.append_nil _⟩
-  (Provable.ax_self axs (.tail _ <| .tail _ <| .head _)).thm
-    (subst.ok.cons vt t.ty $ subst.ok.cons vr r.ty subst.ok.nil)
-    DJ_nil HH_nil⟩
+    Typed "wff" (eq t r) :=
+  ⟨fun _Γ =>
+    have : Subst (subst_of [(vt, t), (vr, r)]) vt t := ⟨List.append_nil _⟩
+    have : Subst (subst_of [(vt, t), (vr, r)]) vr r := ⟨List.append_nil _⟩
+    (Provable.ax_self axs (.tail _ <| .tail _ <| .head _)).thm
+      (subst.ok.cons vt t.ty $ subst.ok.cons vr r.ty subst.ok.nil)
+      DJ_nil HH_nil⟩
 
 instance wim {P Q} [Typed "wff" P] [Typed "wff" Q] :
-  Typed "wff" (im P Q) :=
-⟨fun _Γ =>
-  have : Subst (subst_of [(vP, P), (vQ, Q)]) vP P := ⟨List.append_nil _⟩
-  have : Subst (subst_of [(vP, P), (vQ, Q)]) vQ Q := ⟨List.append_nil _⟩
-  (Provable.ax_self axs (.tail _ <| .tail _ <| .tail _ <| .head _)).thm
-    (subst.ok.cons vP P.ty $ subst.ok.cons vQ Q.ty subst.ok.nil)
-    DJ_nil HH_nil⟩
+    Typed "wff" (im P Q) :=
+  ⟨fun _Γ =>
+    have : Subst (subst_of [(vP, P), (vQ, Q)]) vP P := ⟨List.append_nil _⟩
+    have : Subst (subst_of [(vP, P), (vQ, Q)]) vQ Q := ⟨List.append_nil _⟩
+    (Provable.ax_self axs (.tail _ <| .tail _ <| .tail _ <| .head _)).thm
+      (subst.ok.cons vP P.ty $ subst.ok.cons vQ Q.ty subst.ok.nil)
+      DJ_nil HH_nil⟩
 
 instance wal {x P} [Typed "set" x] [Typed "wff" P] :
-  Typed "wff" (al x P) :=
-⟨fun _Γ =>
-  have : Subst (subst_of [(vx, x), (vP, P)]) vx x := ⟨List.append_nil _⟩
-  have : Subst (subst_of [(vx, x), (vP, P)]) vP P := ⟨List.append_nil _⟩
-  (Provable.ax_self axs (.tail _ <| .tail _ <| .tail _ <| .tail _ <| .head _)).thm
-    (subst.ok.cons vx x.ty $ subst.ok.cons vP P.ty subst.ok.nil)
-    DJ_nil HH_nil⟩
+    Typed "wff" (al x P) :=
+  ⟨fun _Γ =>
+    have : Subst (subst_of [(vx, x), (vP, P)]) vx x := ⟨List.append_nil _⟩
+    have : Subst (subst_of [(vx, x), (vP, P)]) vP P := ⟨List.append_nil _⟩
+    (Provable.ax_self axs (.tail _ <| .tail _ <| .tail _ <| .tail _ <| .head _)).thm
+      (subst.ok.cons vx x.ty $ subst.ok.cons vP P.ty subst.ok.nil)
+      DJ_nil HH_nil⟩
 
 theorem a1 {Γ t r s} [Typed "term" t] [Typed "term" r] [Typed "term" s] :
-  Provable Γ ("|-", im (eq t r) (im (eq t s) (eq r s))) :=
+    Provable Γ ("|-", im (eq t r) (im (eq t s) (eq r s))) :=
   have : Subst (subst_of [(vt, t), (vr, r), (vs, s)]) vt t := ⟨List.append_nil _⟩
   have : Subst (subst_of [(vt, t), (vr, r), (vs, s)]) vr r := ⟨List.append_nil _⟩
   have : Subst (subst_of [(vt, t), (vr, r), (vs, s)]) vs s := ⟨List.append_nil _⟩
@@ -515,16 +515,16 @@ theorem a1 {Γ t r s} [Typed "term" t] [Typed "term" r] [Typed "term" s] :
     DJ_nil HH_nil
 
 theorem a2 {Γ t} [Typed "term" t] :
-  Provable Γ ("|-", eq (pl t ze) t) :=
+    Provable Γ ("|-", eq (pl t ze) t) :=
   have : Subst (subst_of [(vt, t)]) vt t := ⟨List.append_nil _⟩
   (Provable.ax_self axs (.tail _ <| .tail _ <| .tail _ <| .tail _ <| .tail _ <| .tail _ <| .head _)).thm
     (subst.ok.cons vt t.ty subst.ok.nil)
     DJ_nil HH_nil
 
 theorem mp {Γ P Q} [Typed "wff" P] [Typed "wff" Q]
-  (min : Provable Γ ("|-", P))
-  (maj : Provable Γ ("|-", im P Q)) :
-  Provable Γ ("|-", Q) :=
+    (min : Provable Γ ("|-", P))
+    (maj : Provable Γ ("|-", im P Q)) :
+    Provable Γ ("|-", Q) :=
   have : Subst (subst_of [(vP, P), (vQ, Q)]) vP P := ⟨List.append_nil _⟩
   have : Subst (subst_of [(vP, P), (vQ, Q)]) vQ Q := ⟨List.append_nil _⟩
   (Provable.ax_self axs (.tail _ <| .tail _ <| .tail _ <| .tail _ <| .tail _ <| .tail _ <| .tail _ <| .head _)).thm
@@ -532,8 +532,8 @@ theorem mp {Γ P Q} [Typed "wff" P] [Typed "wff" Q]
     DJ_nil (HH_cons min $ HH_cons maj HH_nil)
 
 theorem ax5 {Γ x P} [Typed "set" x] [Typed "wff" P]
-  (xp : x.disjoint Γ.dj P) :
-  Provable Γ ("|-", im P (al x P)) :=
+    (xp : x.disjoint Γ.dj P) :
+    Provable Γ ("|-", im P (al x P)) :=
   have : Subst (subst_of [(vx, x), (vP, P)]) vx x := ⟨List.append_nil _⟩
   have : Subst (subst_of [(vx, x), (vP, P)]) vP P := ⟨List.append_nil _⟩
   (Provable.ax_self axs (.tail _ <| .tail _ <| .tail _ <| .tail _ <| .tail _ <| .tail _ <| .tail _ <| .tail _ <| .head _)).thm
