Metamath.lean
@@ -2,7 +2,7 @@ import Metamath.Verify
 
 open Metamath.Verify in
 def main (n : List String) : IO UInt32 := do
-  let db ← check $ n.getD 0 "set.mm"
+  let db ← check <| n.getD 0 "set.mm"
   match db.error? with
   | none =>
     IO.println s!"verified, {db.objects.size} objects"
